Finished liveness impl

ticket_states.dfy
@@ -9,7 +9,7 @@ datatype State = State(nextTicket: int, serving: int, controlStates: map<Process
 
 const processes: set<Process>
 
-ghost predicate Valid(s: State)
+predicate Valid(s: State)
 {
   && s.controlStates.Keys == s.tickets.Keys == processes
   && (forall p, q :: 
@@ -18,4 +18,71 @@ ghost predicate Valid(s: State)
   && s.nextTicket >= s.serving
   && (forall p :: p in processes && s.controlStates[p] != Thinking ==> s.serving <= s.tickets[p] < s.nextTicket)
   && (forall p :: p in processes && s.controlStates[p] == Eating ==> s.tickets[p] == s.serving)
+}
+
+lemma MutualExlusion(s: State, p: Process, q: Process)
+  requires Valid(s)
+  requires p in processes && q in processes 
+  requires s.controlStates[p] == s.controlStates[q] == Eating
+  ensures p == q 
+{
+}
+
+predicate Init(s: State)
+{
+  && s.controlStates.Keys == s.tickets.Keys == processes
+  && s.nextTicket == s.serving
+  && (forall p :: p in processes ==> s.controlStates[p] == Thinking)
+}
+
+predicate Next(s: State, s': State)
+{
+  && Valid(s)
+  && exists p :: p in processes && NextP(s, p, s')
+}
+
+lemma Invariance(s: State, s': State)
+  ensures Init(s) ==> Valid(s)
+  ensures Valid(s) && Next(s, s') ==> Valid(s')
+{
+}
+
+predicate NextP(s: State, p: Process, s': State)
+  requires Valid(s) && p in processes
+{
+  || Request(s, p, s')
+  || Enter(s, p, s')
+  || Leave(s, p, s')
+}
+
+predicate Request(s: State, p: Process, s': State)
+  requires Valid(s) && p in processes
+{
+  && s.controlStates[p] == Thinking
+  && s'.nextTicket == s.nextTicket + 1
+  && s'.tickets == s.tickets[p := s.nextTicket] 
+  && s'.serving == s.serving
+  && s'.controlStates == s.controlStates[p := Hungry]
+}
+
+predicate Enter(s: State, p: Process, s': State)
+  requires Valid(s) && p in processes
+{
+  && s.controlStates[p] == Hungry 
+  && s.tickets[p] == s.serving
+  && s'.tickets == s.tickets 
+  && s'.nextTicket == s.nextTicket
+  && s'.serving == s.serving
+  && ((s.tickets[p] == s.serving && s'.controlStates == s.controlStates[p := Eating]) ||
+      (s.tickets[p] != s.serving && s'.controlStates == s.controlStates))
+}
+
+predicate Leave(s: State, p: Process, s': State)
+  requires Valid(s) && p in processes
+{
+  && s.controlStates[p] == Eating
+  && s'.nextTicket == s.nextTicket
+  && s'.tickets == s.tickets 
+  && s'.serving == s.serving + 1
+  && s'.controlStates == s.controlStates[p := Thinking]
 }
